Phi_Semantics/PhiSem_CF_Basic.thy
@@ -1,6 +1,6 @@
 chapter \<open>Basic Control Flow\<close>
 
-theory PhiSem_Basic_Control_Flow
+theory PhiSem_CF_Basic
   imports PhiSem_Generic_Boolean
 begin
 
@@ -159,10 +159,11 @@ proc while:
   assumes \<open>\<^bold>p\<^bold>a\<^bold>r\<^bold>a\<^bold>m ( X x \<^bold>s\<^bold>u\<^bold>b\<^bold>j x. Inv: invariant x \<and> Guard: cond x)\<close>
   assumes V[unfolded Action_Tag_def]:
            "\<^bold>v\<^bold>i\<^bold>e\<^bold>w X' \<longmapsto> (X x \<^bold>s\<^bold>u\<^bold>b\<^bold>j x. invariant x) \<^bold>w\<^bold>i\<^bold>t\<^bold>h Any @action ToSA"
-    and C: "\<forall>x. \<^bold>p\<^bold>r\<^bold>e\<^bold>m\<^bold>i\<^bold>s\<^bold>e invariant x \<longrightarrow> \<^bold>p\<^bold>r\<^bold>o\<^bold>c Cond \<lbrace> X x \<longmapsto> X x'\<heavy_comma> \<^bold>v\<^bold>a\<^bold>l cond x' \<Ztypecolon> \<bool> \<^bold>s\<^bold>u\<^bold>b\<^bold>j x'. invariant x' \<rbrace>"
-    and B: "\<forall>x. \<^bold>p\<^bold>r\<^bold>e\<^bold>m\<^bold>i\<^bold>s\<^bold>e invariant x \<longrightarrow> \<^bold>p\<^bold>r\<^bold>e\<^bold>m\<^bold>i\<^bold>s\<^bold>e cond x \<longrightarrow> \<^bold>p\<^bold>r\<^bold>o\<^bold>c Body \<lbrace> X x \<longmapsto> X x' \<^bold>s\<^bold>u\<^bold>b\<^bold>j x'. invariant x' \<rbrace>"
+    and C: "\<forall>x. \<^bold>p\<^bold>r\<^bold>e\<^bold>m\<^bold>i\<^bold>s\<^bold>e invariant x \<longrightarrow> \<^bold>p\<^bold>r\<^bold>o\<^bold>c Cond \<lbrace> X x \<longmapsto> X x'\<heavy_comma> \<^bold>v\<^bold>a\<^bold>l cond x' \<Ztypecolon> \<bool> \<^bold>s\<^bold>u\<^bold>b\<^bold>j x'. invariant x' \<rbrace> \<^bold>t\<^bold>h\<^bold>r\<^bold>o\<^bold>w\<^bold>s E1"
+    and B: "\<forall>x. \<^bold>p\<^bold>r\<^bold>e\<^bold>m\<^bold>i\<^bold>s\<^bold>e invariant x \<longrightarrow> \<^bold>p\<^bold>r\<^bold>e\<^bold>m\<^bold>i\<^bold>s\<^bold>e cond x \<longrightarrow> \<^bold>p\<^bold>r\<^bold>o\<^bold>c Body \<lbrace> X x \<longmapsto> X x' \<^bold>s\<^bold>u\<^bold>b\<^bold>j x'. invariant x' \<rbrace> \<^bold>t\<^bold>h\<^bold>r\<^bold>o\<^bold>w\<^bold>s E2"
   input  \<open>X'\<close>
   output \<open>X x \<^bold>s\<^bold>u\<^bold>b\<^bold>j x. invariant x \<and> \<not> cond x\<close>
+  throws \<open>E1 + E2\<close>
   \<medium_left_bracket> V C
     branch \<medium_left_bracket>
       do_while \<open>X vars \<^bold>s\<^bold>u\<^bold>b\<^bold>j vars. Inv: invariant vars \<and> Guard: cond vars\<close>
