Phi_Semantics/PhiSem_CF_Breakable.thy
@@ -1,0 +1,42 @@
+theory PhiSem_CF_Breakable
+  imports PhiSem_CF_Break PhiSem_CF_Basic
+begin
+
+thm while_\<phi>app
+
+definition continue_label :: \<open>brk_label \<Rightarrow> brk_label\<close>
+  where \<open>continue_label x = x\<close>
+
+thm brk_scope
+
+declare [[\<phi>display_brk_frame]]
+declare [[\<phi>trace_reasoning]]
+
+proc while:
+  assumes \<open>\<^bold>p\<^bold>a\<^bold>r\<^bold>a\<^bold>m (X x \<^bold>s\<^bold>u\<^bold>b\<^bold>j x. Inv: invariant x \<and> Guard: cond x)\<close>
+  and CT: \<open>\<^bold>v\<^bold>i\<^bold>e\<^bold>w U \<longmapsto> (X x \<^bold>s\<^bold>u\<^bold>b\<^bold>j x. invariant x) @action ToSA\<close>
+  and C: "\<And>x. \<^bold>p\<^bold>r\<^bold>e\<^bold>m\<^bold>i\<^bold>s\<^bold>e invariant x \<Longrightarrow>
+                  \<^bold>p\<^bold>r\<^bold>o\<^bold>c Cond \<lbrace> X x \<longmapsto> X x'\<heavy_comma> \<^bold>v\<^bold>a\<^bold>l cond x' \<Ztypecolon> \<bool> \<^bold>s\<^bold>u\<^bold>b\<^bold>j x'. invariant x' \<rbrace> \<^bold>t\<^bold>h\<^bold>r\<^bold>o\<^bold>w\<^bold>s E1"
+  and B: "\<And>x lb lc. \<^bold>p\<^bold>r\<^bold>e\<^bold>m\<^bold>i\<^bold>s\<^bold>e invariant x \<Longrightarrow>
+                    \<^bold>p\<^bold>r\<^bold>e\<^bold>m\<^bold>i\<^bold>s\<^bold>e cond x \<Longrightarrow>
+                    \<^bold>p\<^bold>r\<^bold>o\<^bold>c Body \<lbrace> X x\<heavy_comma> Brk_Frame (continue_label lc)\<heavy_comma> Brk_Frame lb
+                            \<longmapsto> X x'\<heavy_comma> Brk_Frame (continue_label lc)\<heavy_comma> Brk_Frame lb
+                                \<^bold>s\<^bold>u\<^bold>b\<^bold>j x'. invariant x'
+                              \<rbrace> \<^bold>t\<^bold>h\<^bold>r\<^bold>o\<^bold>w\<^bold>s (\<lambda>e. \<^bold>b\<^bold>r\<^bold>e\<^bold>a\<^bold>k lb \<^bold>w\<^bold>i\<^bold>t\<^bold>h (\<lambda>_. X x'\<heavy_comma> Brk_Frame (continue_label lc) \<^bold>s\<^bold>u\<^bold>b\<^bold>j x'. invariant x \<and> \<not> cond x)
+                                         \<^bold>o\<^bold>r \<^bold>b\<^bold>r\<^bold>e\<^bold>a\<^bold>k (continue_label lc) \<^bold>w\<^bold>i\<^bold>t\<^bold>h (\<lambda>_. X x'\<heavy_comma> Brk_Frame lb \<^bold>s\<^bold>u\<^bold>b\<^bold>j x'. invariant x)
+                                         \<^bold>o\<^bold>r E2 e)"
+  input \<open>U\<close>
+  output \<open>X x \<^bold>s\<^bold>u\<^bold>b\<^bold>j x. invariant x \<and> \<not> cond x\<close>
+  \<medium_left_bracket> CT
+    brk_scope \<medium_left_bracket> for lb
+      PhiSem_CF_Basic.while \<open>Brk_Frame lb\<heavy_comma> X x \<^bold>s\<^bold>u\<^bold>b\<^bold>j x. Inv: invariant x \<and> Guard: cond x\<close>
+      \<medium_left_bracket> C \<medium_right_bracket>.
+      \<medium_left_bracket> brk_scope \<medium_left_bracket> for lc
+        have wrap: \<open>Brk_Frame lc = Brk_Frame (continue_label lc)\<close> unfolding continue_label_def ..
+        ;; unfold wrap
+           B \<exists>x'
+           fold wrap
+        \<medium_right_bracket>
+        ..
+
+end
